---
title: "ORIE4742_HW1"
output: html_document
---

```{r setup, include=FALSE}
knitr::opts_chunk$set(echo = TRUE)
```

1.

a)

i)

For an infinite sum:

$$
\sum_{n=1}^{\infty} a_1 r^{n-1} = \frac{a_1}{1-r}
$$
So:

$$
\sum_{n=1}^{\infty} e^{-2n}
$$
$$
= \frac{1}{e^2 -1}
$$
ii)

$$
\int_0^{\infty} e^{-x^2 /2} dx
$$
Substituting:

$$
u = x / \sqrt{2}
$$
$$
du/dx = 1/\sqrt{2}
$$
So:

$$
\int_0^{\infty} e^{-x^2 /2} dx = \sqrt{\frac{\pi}{2}} \int_0^{\infty} \frac{2e^{-u^2}}{\sqrt{\pi}} du = \sqrt{\frac{\pi}{2}} \mbox{erf}(u) |_0^{\infty}
$$
$$
= \sqrt{\frac{\pi}{2}} \mbox{erf}(\frac{x}{\sqrt{2}}) |_0^{\infty} = \sqrt{\frac{\pi}{2}}
$$

iii)

$$
\sum_{n=1}^{\infty} \frac{1}{n(n+1)}
$$
$$
= \sum_{n=1}^{\infty} (\frac{1}{n} - \frac{1}{n+1})
$$
$$
\sum_{n=1}^m (\frac{1}{n} - \frac{1}{n+1}) = 1 - \frac{1}{2} + \frac{1}{2} - \frac{1}{3} + \frac{1}{3} + \dots - \frac{1}{m} + \frac{1}{m} - \frac{1}{m+1}
$$
So as $m$ goes to infinity:

$$
\sum_{n=1}^{\infty} \frac{1}{n(n+1)} = 1
$$

iv)

$$
\sum_{n=1}^{\infty} \frac{1}{n^2} = 1 + \frac{1}{4} + \frac{1}{9} + \frac{1}{16} + \dots + \frac{1}{n^2} = \frac{\pi^2}{6}
$$
So

$$
\sum_{n=1}^{\infty} \frac{1}{n^2} \in (1,2)
$$

b)

Showing this empirically by choosing $n = 5$:

$$
\int_1^6 \frac{1}{x} dx = \mbox{ln}(x) |_1^6 = \mbox{ln}(6) - \mbox{ln}(1) = 1.79
$$
$$
H_5 = \sum_{i=1}^5 \frac{1}{i} = 2.28
$$
$$
1 + \int_1^5 \frac{1}{x} dx = 2.61
$$
We see:

$$
\int_1^6 \frac{1}{x} dx < H_5 < 1 + \int_1^5 \frac{1}{x} dx
$$
More formally:

$$
\int_1^{n+1} \frac{1}{x} dx \le H_n \le 1 + \int_1^n \frac{1}{x} dx
$$
Equivalent to:

$$
\mbox{ln}(n+1) \le H_n \le 1 + \mbox{ln}(x)
$$
If we take the upper bound $x \in [i,i+1)$ then

$$
H_n \ge \int_1^{n+1} \frac{1}{x} dx
$$
If we take the lower bound $x \in (i-1,i]$ then 

$$
H_n \le 1 + \int_1^n \frac{1}{x} dx
$$

c)

Noting that:

$$
\mbox{ln}(n!) = \sum_{i=2}^n \mbox{ln}(i)
$$

If we take the upper bound $x \in [i,i+1)$ then

$$
\int_1^{n+1} \mbox{ln}(x)dx = (x\mbox{ln}(x) - x)|_1^{n+1} = (n+1)\mbox{ln}(n+1) - n
$$
$$
\ge \mbox{ln}(n!)
$$
If we take the lower bound $x \in (i-1,i]$ then

$$
\int_1^{n} \mbox{ln}(x)dx = (x\mbox{ln}(x) - x)|_1^{n} = n\mbox{ln}(n) - n + 1
$$
$$
\le \mbox{ln}(n!)
$$




